<?xml version="1.0"?>


<!DOCTYPE rdf:RDF [
    <!ENTITY owl "http://www.w3.org/2002/07/owl#" >
    <!ENTITY xsd "http://www.w3.org/2001/XMLSchema#" >
    <!ENTITY rdfs "http://www.w3.org/2000/01/rdf-schema#" >
    <!ENTITY rdf "http://www.w3.org/1999/02/22-rdf-syntax-ns#" >
]>


<rdf:RDF xmlns="http://www.daml.org/services/owl-s/1.2/Service.owl#"
     xml:base="http://www.daml.org/services/owl-s/1.2/Service.owl"
     xmlns:rdfs="http://www.w3.org/2000/01/rdf-schema#"
     xmlns:owl="http://www.w3.org/2002/07/owl#"
     xmlns:xsd="http://www.w3.org/2001/XMLSchema#"
     xmlns:rdf="http://www.w3.org/1999/02/22-rdf-syntax-ns#">
    <owl:Ontology rdf:about="http://www.daml.org/services/owl-s/1.2/Service.owl">
        <rdfs:comment>
    Top level of OWL ontology for services.
    Part of the OWL-S ontology; see http://www.daml.org/services/.  
  </rdfs:comment>
        <owl:versionInfo>
    $Id: Service.owl,v 1.25 2005/05/18 21:45:19 martin Exp $
  </owl:versionInfo>
        <owl:imports rdf:resource="http://www.daml.org/services/owl-s/1.2/Grounding.owl"/>
        <owl:imports rdf:resource="http://www.daml.org/services/owl-s/1.2/Process.owl"/>
        <owl:imports rdf:resource="http://www.daml.org/services/owl-s/1.2/Profile.owl"/>
    </owl:Ontology>
    


    <!-- 
    ///////////////////////////////////////////////////////////////////////////////////////
    //
    // Annotation properties
    //
    ///////////////////////////////////////////////////////////////////////////////////////
     -->

    


    <!-- 
    ///////////////////////////////////////////////////////////////////////////////////////
    //
    // Datatypes
    //
    ///////////////////////////////////////////////////////////////////////////////////////
     -->

    


    <!-- 
    ///////////////////////////////////////////////////////////////////////////////////////
    //
    // Object Properties
    //
    ///////////////////////////////////////////////////////////////////////////////////////
     -->

    


    <!-- http://www.daml.org/services/owl-s/1.2/Service.owl#describedBy -->

    <owl:ObjectProperty rdf:about="http://www.daml.org/services/owl-s/1.2/Service.owl#describedBy">
        <rdfs:domain rdf:resource="http://www.daml.org/services/owl-s/1.2/Service.owl#Service"/>
        <rdfs:range rdf:resource="http://www.daml.org/services/owl-s/1.2/Service.owl#ServiceModel"/>
    </owl:ObjectProperty>
    


    <!-- http://www.daml.org/services/owl-s/1.2/Service.owl#describes -->

    <owl:ObjectProperty rdf:about="http://www.daml.org/services/owl-s/1.2/Service.owl#describes">
        <rdfs:comment> 
    There are no cardinality restrictions on this property. That is,
    the same service model can be used by many different services.
  </rdfs:comment>
        <rdfs:range rdf:resource="http://www.daml.org/services/owl-s/1.2/Service.owl#Service"/>
        <rdfs:domain rdf:resource="http://www.daml.org/services/owl-s/1.2/Service.owl#ServiceModel"/>
        <owl:inverseOf rdf:resource="http://www.daml.org/services/owl-s/1.2/Service.owl#describedBy"/>
    </owl:ObjectProperty>
    


    <!-- http://www.daml.org/services/owl-s/1.2/Service.owl#presentedBy -->

    <owl:ObjectProperty rdf:about="http://www.daml.org/services/owl-s/1.2/Service.owl#presentedBy">
        <rdfs:comment> 
    There are no cardinality restrictions on this property. 
  </rdfs:comment>
        <rdfs:range rdf:resource="http://www.daml.org/services/owl-s/1.2/Service.owl#Service"/>
        <rdfs:domain rdf:resource="http://www.daml.org/services/owl-s/1.2/Service.owl#ServiceProfile"/>
        <owl:inverseOf rdf:resource="http://www.daml.org/services/owl-s/1.2/Service.owl#presents"/>
    </owl:ObjectProperty>
    


    <!-- http://www.daml.org/services/owl-s/1.2/Service.owl#presents -->

    <owl:ObjectProperty rdf:about="http://www.daml.org/services/owl-s/1.2/Service.owl#presents">
        <rdfs:comment> 
    There are no cardinality restrictions on this property. 
  </rdfs:comment>
        <rdfs:domain rdf:resource="http://www.daml.org/services/owl-s/1.2/Service.owl#Service"/>
        <rdfs:range rdf:resource="http://www.daml.org/services/owl-s/1.2/Service.owl#ServiceProfile"/>
    </owl:ObjectProperty>
    


    <!-- http://www.daml.org/services/owl-s/1.2/Service.owl#providedBy -->

    <owl:ObjectProperty rdf:about="http://www.daml.org/services/owl-s/1.2/Service.owl#providedBy">
        <rdfs:domain rdf:resource="http://www.daml.org/services/owl-s/1.2/Service.owl#Service"/>
        <owl:inverseOf rdf:resource="http://www.daml.org/services/owl-s/1.2/Service.owl#provides"/>
    </owl:ObjectProperty>
    


    <!-- http://www.daml.org/services/owl-s/1.2/Service.owl#provides -->

    <owl:ObjectProperty rdf:about="http://www.daml.org/services/owl-s/1.2/Service.owl#provides">
        <rdfs:comment>
    OWL-S is completely agnostic at present about what kind of thing
    provides a service (hence, no domain declared here).
  </rdfs:comment>
        <rdfs:range rdf:resource="http://www.daml.org/services/owl-s/1.2/Service.owl#Service"/>
    </owl:ObjectProperty>
    


    <!-- http://www.daml.org/services/owl-s/1.2/Service.owl#supportedBy -->

    <owl:ObjectProperty rdf:about="http://www.daml.org/services/owl-s/1.2/Service.owl#supportedBy">
        <rdfs:range rdf:resource="http://www.daml.org/services/owl-s/1.2/Service.owl#Service"/>
        <rdfs:domain rdf:resource="http://www.daml.org/services/owl-s/1.2/Service.owl#ServiceGrounding"/>
        <owl:inverseOf rdf:resource="http://www.daml.org/services/owl-s/1.2/Service.owl#supports"/>
    </owl:ObjectProperty>
    


    <!-- http://www.daml.org/services/owl-s/1.2/Service.owl#supports -->

    <owl:ObjectProperty rdf:about="http://www.daml.org/services/owl-s/1.2/Service.owl#supports">
        <rdfs:domain rdf:resource="http://www.daml.org/services/owl-s/1.2/Service.owl#Service"/>
        <rdfs:range rdf:resource="http://www.daml.org/services/owl-s/1.2/Service.owl#ServiceGrounding"/>
    </owl:ObjectProperty>
    


    <!-- 
    ///////////////////////////////////////////////////////////////////////////////////////
    //
    // Classes
    //
    ///////////////////////////////////////////////////////////////////////////////////////
     -->

    


    <!-- http://www.daml.org/services/owl-s/1.2/Service.owl#Service -->

    <owl:Class rdf:about="http://www.daml.org/services/owl-s/1.2/Service.owl#Service">
        <rdfs:label>Service</rdfs:label>
        <rdfs:subClassOf>
            <owl:Restriction>
                <owl:onProperty rdf:resource="http://www.daml.org/services/owl-s/1.2/Service.owl#describedBy"/>
                <owl:maxCardinality rdf:datatype="&xsd;nonNegativeInteger">1</owl:maxCardinality>
            </owl:Restriction>
        </rdfs:subClassOf>
        <rdfs:comment>See comments above</rdfs:comment>
        <rdfs:comment> 
    A service has 0 or 1 models.  (But note that a service with 0 models 
    does not provide automated online access; it exists only for
    discovery purposes; that is, it exists so as to provide a Profile.)
  </rdfs:comment>
    </owl:Class>
    


    <!-- http://www.daml.org/services/owl-s/1.2/Service.owl#ServiceGrounding -->

    <owl:Class rdf:about="http://www.daml.org/services/owl-s/1.2/Service.owl#ServiceGrounding">
        <rdfs:label>ServiceGrounding</rdfs:label>
        <rdfs:subClassOf>
            <owl:Restriction>
                <owl:onProperty rdf:resource="http://www.daml.org/services/owl-s/1.2/Service.owl#supportedBy"/>
                <owl:cardinality rdf:datatype="&xsd;nonNegativeInteger">1</owl:cardinality>
            </owl:Restriction>
        </rdfs:subClassOf>
        <rdfs:comment>See comments above</rdfs:comment>
        <rdfs:comment> 
    A Grounding must be associated with exactly one service.
    (Also, that service must have a model - but that constraint
    isn&apos;t expressed here.)
  </rdfs:comment>
    </owl:Class>
    


    <!-- http://www.daml.org/services/owl-s/1.2/Service.owl#ServiceModel -->

    <owl:Class rdf:about="http://www.daml.org/services/owl-s/1.2/Service.owl#ServiceModel">
        <rdfs:label>ServiceModel</rdfs:label>
        <rdfs:comment>See comments above</rdfs:comment>
    </owl:Class>
    


    <!-- http://www.daml.org/services/owl-s/1.2/Service.owl#ServiceProfile -->

    <owl:Class rdf:about="http://www.daml.org/services/owl-s/1.2/Service.owl#ServiceProfile">
        <rdfs:label>ServiceProfile</rdfs:label>
        <rdfs:comment>See comments above</rdfs:comment>
    </owl:Class>
</rdf:RDF>



<!-- Generated by the OWL API (version 3.3.1957) http://owlapi.sourceforge.net -->

